some backup of rather uniform proofs.

SEARwfun.sml
@@ -46,3 +46,113 @@ fun ind_with th (ct,asl,w) =
         val th1 = fVar_Inst_th (P,(bvs,b)) th
     in match_mp_tac th1 (ct,asl,w)
     end
+
+
+
+val _ = new_sort "set" [];
+val _ = new_sort "mem" [("A",mk_sort "set" [])];
+val _ = new_sort "rel" [("A",mk_sort "set" []),("B",mk_sort "set" [])]
+val _ = new_sort_infix "rel" "->"
+
+val set_sort = mk_sort "set" []
+fun mem_sort A = mk_sort "mem" [A]
+fun rel_sort A B = mk_sort "rel" [A,B]
+fun mk_set A = mk_var(A,set_sort)
+fun mk_rel R A B = mk_var(R,rel_sort A B)
+fun mk_mem a A = mk_var(a,mem_sort A)
+
+val _ = EqSorts := "rel" :: (!EqSorts)
+val _ = EqSorts := "mem" :: (!EqSorts)
+
+val _ = new_pred "Holds" [("R",rel_sort (mk_set "A") (mk_set "B")),
+                         ("a",mem_sort (mk_set "A")),
+                         ("b",mem_sort (mk_set "B"))]
+
+
+
+fun eq_sym a = 
+    if mem a (!EqSorts) then 
+        let val ns0 = srt2ns a
+            val v1 = mk_var ns0
+            val v2 = pvariantt (HOLset.add(essps,ns0)) v1
+            val v1v2 = mk_eq v1 v2
+            val v2v1 = mk_eq v2 v1
+            val l2r = assume v1v2 |> sym|> disch_all
+            val r2l = assume v2v1 |> sym|> disch_all
+        in dimpI l2r r2l
+        end
+    else raise ERR ("eq_sym.input sort: " ^ a ^ " does not have equality",
+                    [],[],[])
+
+
+
+val lflip_tac =
+fconv_tac 
+ (land_fconv no_conv 
+ $ basic_once_fconv no_conv
+ (first_fconv (List.map (rewr_fconv o eq_sym) (!EqSorts))))
+
+ 
+
+val rflip_tac =
+fconv_tac 
+ (rand_fconv no_conv 
+ $ basic_once_fconv no_conv
+ (first_fconv (List.map (rewr_fconv o eq_sym) (!EqSorts))))
+
+
+
+val flip_tac = 
+fconv_tac 
+ (basic_once_fconv no_conv 
+  (first_fconv (List.map (rewr_fconv o eq_sym) (!EqSorts))))
+
+
+
+val _ = new_sort "set" [];
+val _ = new_sort "mem" [("A",mk_sort "set" [])];
+val _ = new_sort "rel" [("A",mk_sort "set" []),("B",mk_sort "set" [])]
+val _ = new_sort_infix "rel" "->"
+
+val set_sort = mk_sort "set" []
+fun mem_sort A = mk_sort "mem" [A]
+fun rel_sort A B = mk_sort "rel" [A,B]
+fun mk_set A = mk_var(A,set_sort)
+fun mk_rel R A B = mk_var(R,rel_sort A B)
+fun mk_mem a A = mk_var(a,mem_sort A)
+
+val _ = EqSorts := "rel" :: (!EqSorts)
+val _ = EqSorts := "mem" :: (!EqSorts)
+
+val _ = new_pred "Holds" [("R",rel_sort (mk_set "A") (mk_set "B")),
+                         ("a",mem_sort (mk_set "A")),
+                         ("b",mem_sort (mk_set "B"))]
+
+val Fun_def = define_pred “!A B R:rel(A,B). isFun(R) <=> !x:mem(A). ?!y:mem(B). Holds(R,x,y)”
+
+
+val Fun_expand = prove_store("Fun_expand",
+e0
+(rpt strip_tac >> rw[Fun_def] >>
+ rw[uex_def “?!y:mem(B).Holds(R,x,y)”] >> 
+ dimp_tac >> strip_tac (* 2 *)
+ >-- (rpt strip_tac (* 2 *)
+     >-- (first_x_assum (qspecl_then [‘a’] assume_tac) >> 
+          pop_assum strip_assume_tac >> qexists_tac ‘y’ >> arw[]) 
+     >-- (first_x_assum (qspecl_then [‘a’] strip_assume_tac) >>
+          first_assum rev_drule >>
+          first_assum (qspecl_then [‘b2’] assume_tac) >>
+          first_assum drule >> arw[])) >>
+ rpt strip_tac >> last_x_assum (qspecl_then [‘x’] strip_assume_tac) >>
+ qexists_tac ‘b’ >> arw[] >> rpt strip_tac >> first_x_assum irule >>
+ qexists_tac ‘x’ >> arw[])
+(form_goal
+“!A B R:A->B. isFun(R) <=>
+ (!a.?b.Holds(R,a,b)) & 
+ (!a b1 b2. Holds(R,a,b1) & Holds(R,a,b2) ==> b1 = b2)”));
+
+val _ = new_fun "Eval" (mem_sort (mk_set "B"),[("R",rel_sort (mk_set "A") (mk_set "B")),
+                        ("x",mem_sort (mk_set "A"))]) 
+
+val Eval_def = new_ax “!A B Fn:rel(A,B). isFun(Fn) ==>!x y. Holds(Fn,x,y) <=> y = Eval(Fn,x)”
+
