relnbyhand.sml
@@ -1,0 +1,615 @@
+val AX4 = new_ax
+“?N0 O0:mem(N0) S0:N0->N0. isFun(S0) & (!n:mem(N0). ~(Eval(S0,n) = O0)) & 
+ !n m. Eval(S0,n) = Eval(S0,m) <=> n = m”
+
+(*is it fair to add the constriction that no formula variable can occur in the input of define_pred, if not, we can write:
+!n. inN(n) <=> 
+    P(n0) &
+    (!n0. P(n0) ==> P(Eval(S0,n0))) ==>
+    P(n)
+
+think a problem is that if we allow the definition to include fvars,
+then we can make something like:
+
+|- !n. inN(n) <=> P(n) as a thm
+
+and inst the P(n) to be ~inN(n)
+
+this is !n. F. but not equivalent to F. it just says there should be no member such that inN, maybe not problematic, just weird.
+
+*)
+
+fun ind_with th (ct,asl,w) = 
+    let 
+        val th1 = undisch th
+        val (bvs,conc) = dest_forall (concl th1)
+        val (ante,con) = dest_imp conc
+                         handle _ => (TRUE,conc)
+        val (P,args) = dest_fvar con
+        val (b,qvs) = strip_forall w
+        val (gante,gcon) = dest_imp b
+                           handle _ => (TRUE,b)
+        val th2 = fVar_Inst_th (P,(qvs,gcon)) th
+    in match_mp_tac th2 (ct,asl,w)
+    end
+
+fun spec_fVar pdef th = 
+    let val (l,r) = dest_dimp pdef 
+        val (P,vars0) = dest_fvar l
+        val vars = List.map dest_var vars0
+    in fVar_Inst_th (P,(vars,r)) th
+    end
+
+val inN_def = define_pred
+“!n:mem(N0). inN(n) <=>
+(!P.IN(O0,P) &
+ (!n0. IN(n0,P) ==> IN(Eval(S0,n0),P)) ==> 
+ IN(n,P))”
+
+
+val inN_ind0 = 
+    inN_def |> spec_all |> dimpl2r |> undisch
+            |> strip_all_and_imp 
+            |> disch “inN(n)”
+            |> gen_all
+            |> disch_all 
+            |> gen_all
+
+local 
+val l = allE (rastt "N0") IN_def_P_expand
+in
+val inN_ind = prove_store("inN_ind",
+e0
+(strip_tac >> rw[inN_def] >> rpt strip_tac >>
+ qsuff_tac
+ ‘?P0. !n:mem(N0). IN(n,P0) <=> P(n)’
+ >-- (strip_tac >> 
+     first_x_assum (qspecl_then [‘P0’] assume_tac) >>
+     rfs[]) >>
+ strip_assume_tac l >> 
+ qexists_tac ‘s’ >> arw[])
+(form_goal 
+ “(P(O0) &
+   (!n0. P(n0) ==> P(Eval(S0,n0))) ==>
+  !n.inN(n) ==> P(n))”))
+end
+
+val inN_rules = prove_store("inN_rules",
+e0
+(strip_tac >-- (rw[inN_def] >> rpt strip_tac) >>
+ rw[inN_def] >> rpt strip_tac >>
+ first_assum match_mp_tac >> first_x_assum match_mp_tac >> arw[])
+(form_goal
+ “inN(O0) & 
+  (!n. inN(n) ==> inN(Eval(S0,n)))”));
+
+val inN_rules_step = inN_rules |> conjE2
+
+
+(*inN_cases there is a case that rw does not work and do not know why*)
+val inN_cases = prove_store("inN_cases",
+e0
+(strip_tac >> dimp_tac >-- 
+ (qsuff_tac
+ ‘!n0. inN(n0) ==> (n0 = O0 |
+  (?a. n0 = Eval(S0,a) & inN(a)))’
+ >-- (strip_tac >> arw[]) >>
+ ind_with inN_ind >> strip_tac (* 2 *)
+ >-- rw[] >>
+ rpt strip_tac (* 2 *) 
+ >-- (disj2_tac >> arw[] >> qexists_tac ‘O0’ >> rw[inN_rules]) >>
+ disj2_tac >> qexists_tac ‘n0'’ >> rw[] >>
+ arw[] >> match_mp_tac inN_rules_step >> arw[]) >>
+ rpt strip_tac (* 2 *)
+ >-- arw[inN_rules] >>
+ arw[] >> match_mp_tac inN_rules_step >> arw[])
+(form_goal
+ “!n0. inN(n0) <=> (n0 = O0 |
+  (?a. n0 = Eval(S0,a) & inN(a)))”));
+
+
+
+val FI_def = define_pred 
+“!X xs:mem(Pow(X)). FI(xs) <=> 
+ !P. (IN(Empty(X),P) &
+      (!xs. IN(xs,P)==> !x.IN(Ins(x,xs),P))) ==>
+     IN(xs,P)”
+
+
+
+val FI_ind0 = 
+    FI_def |> spec_all |> dimpl2r |> undisch
+            |> strip_all_and_imp 
+            |> disch “FI(xs:mem(Pow(X)))”
+            |> gen_all
+            |> disch_all 
+            |> gen_all
+
+local 
+val l = allE (rastt "Pow(X)") IN_def_P_expand
+in
+val FI_ind = prove_store("FI_ind",
+e0
+(strip_tac >> strip_tac >> rw[FI_def] >> rpt strip_tac >>
+ qsuff_tac
+ ‘?P0. !xs:mem(Pow(X)). IN(xs,P0) <=> P(xs)’
+ >-- (strip_tac >> 
+     first_x_assum (qspecl_then [‘P0’] assume_tac) >>
+     rfs[]) >>
+ strip_assume_tac l >> 
+ qexists_tac ‘s’ >> arw[])
+(form_goal 
+ “!X.(P(Empty(X)) &
+   (!xs. P(xs) ==> !x:mem(X).P(Ins(x,xs)))) ==>
+  !xs:mem(Pow(X)).FI(xs) ==> P(xs)”))
+end
+
+val FI_rules = prove_store("FI_rules",
+e0
+(strip_tac >> strip_tac 
+ >-- (rw[FI_def] >> rpt strip_tac) >>
+ rw[FI_def] >> rpt strip_tac >>
+ first_assum match_mp_tac >> first_x_assum match_mp_tac >> arw[])
+(form_goal
+ “!X. FI(Empty(X))& 
+     (!xs:mem(Pow(X)). FI(xs) ==> !x. FI(Ins(x,xs)))”));
+
+val FI_rules_step = FI_rules |> spec_all |> conjE2
+
+
+val FI_cases = prove_store("FI_cases",
+e0
+(strip_tac >> strip_tac >> dimp_tac >-- 
+ (qsuff_tac
+ ‘!xs. FI(xs) ==> (xs = Empty(X) |
+  (?xs0 x0. xs = Ins(x0,xs0) & FI(xs0)))’
+ >-- (strip_tac >> arw[]) >>
+ ind_with (FI_ind |> allE (rastt "X")) >> strip_tac (* 2 *)
+ >-- rw[] >>
+ rpt strip_tac (* 2 *) 
+ >-- (disj2_tac >> arw[] >> qexistsl_tac [‘Empty(X)’,‘x’] >> 
+     rw[FI_rules]) >>
+ disj2_tac >> (*if arw[] >> here, then does not work*) 
+ qexistsl_tac [‘xs'’,‘x’] >> rw[] >> arw[] >>
+ match_mp_tac FI_rules_step >> arw[]) >>
+ rpt strip_tac (* 2 *)
+ >-- arw[FI_rules] >>
+ arw[] >> match_mp_tac FI_rules_step >> arw[])
+(form_goal
+ “!X xs. FI(xs) <=> (xs = Empty(X) |
+  (?xs0 x0. xs = Ins(x0,xs0) & FI(xs0)))”));
+
+
+
+(*necessary to take a term in product rather then a pair? so Cd has only one argument?*)
+(*
+val Cd_def = define_pred
+“!X xsn:mem(Pow(X) * N). Cd(xsn) <=>
+(!P.IN(Pair(Empty(X),O),P) &
+   (!xsn0 x. IN(xsn0,P) & ~IN(x,Fst(xsn0)) ==> 
+    IN(Pair(Ins(x,Fst(xsn0)),Suc(Snd(xsn0))),P)) ==> 
+ IN(xsn,P))”
+
+if use this, then the cases will be:
+
+Cd(xsn) <=> ?... long. 
+
+*)
+
+val Cd_def = define_pred
+“!X xs:mem(Pow(X)) n. Cd(xs,n) <=>
+(!P.IN(Pair(Empty(X),O),P) &
+   (!xs0 n0 x. IN(Pair(xs0,n0),P) & ~IN(x,xs0) ==>
+   IN(Pair(Ins(x,xs0),Suc(n0)),P)) ==> 
+ IN(Pair(xs,n),P))”
+
+
+val Cd_ind0 = 
+    Cd_def |> spec_all |> dimpl2r |> undisch
+            |> strip_all_and_imp 
+            |> disch “Cd(xs:mem(Pow(X)),n)”
+            |> qgen ‘n’ |> qgen ‘xs’
+            |> disch_all 
+            |> gen_all 
+
+val Fst_of_Pair = prove_store("Fst_of_Pair",
+e0
+(rw[GSYM Fst_def,Eval_p1_Pair])
+(form_goal
+ “!A B a:mem(A) b:mem(B). Fst(Pair(a,b)) = a”));
+
+
+val Snd_of_Pair = prove_store("Snd_of_Pair",
+e0
+(rw[GSYM Snd_def,Eval_p2_Pair])
+(form_goal
+ “!A B a:mem(A) b:mem(B). Snd(Pair(a,b)) = b”));
+
+
+local 
+val l = allE (rastt "Pow(X) * N") IN_def_P_expand |>
+spec_fVar “P(xsn) <=> P(Fst(xsn),Snd(xsn))”
+in
+val Cd_ind = prove_store("Cd_ind",
+e0
+(strip_tac >> rw[Cd_def] >> rpt strip_tac >>
+ qsuff_tac
+ ‘?P0. !xs:mem(Pow(X)) n. IN(Pair(xs,n),P0) <=> P(xs,n)’
+ >-- (strip_tac >> 
+     first_x_assum (qspecl_then [‘P0’] assume_tac) >>
+     rfs[]) >>
+ strip_assume_tac l >> 
+ qexists_tac ‘s’ >> (* simply arw[] works for previous cases but not for this, since the pattern is different *)
+ qby_tac ‘!xs n. P(xs,n) <=> IN(Pair(xs,n),s)’ 
+ >-- (rpt strip_tac >> 
+      first_x_assum (qspecl_then [‘Pair(xs',n')’] assume_tac) >>
+      fs[Fst_of_Pair,Snd_of_Pair]) >>
+ arw[])
+(form_goal 
+ “!X.(P(Empty(X),O) &
+     (!xs n x:mem(X). 
+      P(xs,n) & (~IN(x,xs)) ==> 
+      P(Ins(x,xs),Suc(n)))) ==>
+  !xs:mem(Pow(X)) n.Cd(xs,n) ==> P(xs,n)”))
+end
+
+val Cd_rules = prove_store("Cd_rules",
+e0
+(strip_tac >> strip_tac 
+ >-- (rw[Cd_def] >> rpt strip_tac) >>
+ rw[Cd_def] >> rpt strip_tac >>
+ first_assum match_mp_tac >> arw[] (*to eliminate the ~IN(x,xs) in the goal, previously did not have it*) >> 
+ first_x_assum match_mp_tac >> arw[])
+(form_goal
+ “!X. Cd(Empty(X),O)& 
+     (!xs:mem(Pow(X)) n x. Cd(xs,n) & ~(IN(x,xs)) ==> 
+     Cd(Ins(x,xs),Suc(n)))”));
+
+val Cd_rules_step = Cd_rules |> spec_all |> conjE2
+
+
+val Cd_cases = prove_store("Cd_cases",
+e0
+(strip_tac >> strip_tac >> strip_tac >> dimp_tac >-- 
+ (qsuff_tac
+ ‘!xs n. Cd(xs,n) ==> ((xs = Empty(X) & n = O) |
+  (?xs0 n0 x0. ~(IN(x0,xs0)) & xs = Ins(x0,xs0) & n = Suc(n0) &
+  Cd(xs0,n0)))’
+ >-- (strip_tac >> arw[]) >>
+ ind_with (Cd_ind |> allE (rastt "X")) >> strip_tac (* 2 *)
+ >-- rw[] >>
+ rpt strip_tac (* 2 *) 
+ >-- (disj2_tac >> arw[] >> qexistsl_tac [‘Empty(X)’,‘O’,‘x’] >> 
+     rw[Cd_rules] >> (*previously the rw [..._rules] solve the goal, but here require the condition not in empty*) 
+     rw[Empty_property]) >>
+ disj2_tac >> (*if arw[] >> here, then does not work*) 
+ qexistsl_tac [‘xs'’,‘n'’,‘x’] >> rw[] >> arw[] >>
+ match_mp_tac Cd_rules_step >> arw[]) >>
+ rpt strip_tac (* 2 *)
+ >-- arw[Cd_rules] >>
+ arw[] >> match_mp_tac Cd_rules_step >> arw[])
+(form_goal
+ “!X xs:mem(Pow(X)) n. Cd(xs,n) <=> ((xs = Empty(X) & n = O) |
+  (?xs0 n0 x0. ~(IN(x0,xs0)) & xs = Ins(x0,xs0) & n = Suc(n0) &
+   Cd(xs0,n0)))”));
+
+
+
+
+val isL_def = define_pred 
+“!A nas:mem(Pow(N * A)). isL(nas) <=>
+(!P.IN(Empty(N * A),P) &
+   (!nas0. IN(nas0,P) ==>
+    !a.IN(Ins(Pair(CARD(nas0),a),nas0),P)) ==> 
+ IN(nas,P))”
+
+val isL_ind0 = 
+    isL_def |> spec_all |> dimpl2r |> undisch
+            |> strip_all_and_imp 
+            |> disch “isL(nas:mem(Pow(N * A)))”
+            |> gen_all  
+            |> disch_all 
+            |> gen_all 
+
+
+local 
+val l = allE (rastt "Pow(N * A)") IN_def_P_expand
+in
+val isL_ind = prove_store("isL_ind",
+e0
+(strip_tac >> rw[isL_def] >> rpt strip_tac >>
+ qsuff_tac
+ ‘?P0. !nas:mem(Pow(N * A)). IN(nas,P0) <=> P(nas)’
+ >-- (strip_tac >> 
+     first_x_assum (qspecl_then [‘P0’] assume_tac) >>
+     rfs[]) >>
+ strip_assume_tac l >> 
+ qexists_tac ‘s’ >> arw[])
+(form_goal 
+ “!A.(P(Empty(N * A)) &
+   (!nas. P(nas) ==> !a:mem(A).P(Ins(Pair(CARD(nas),a),nas)))) ==>
+  !nas:mem(Pow(N * A)).isL(nas) ==> P(nas)”))
+end
+
+
+val isL_rules = prove_store("isL_rules",
+e0
+(strip_tac >> strip_tac 
+ >-- (rw[isL_def] >> rpt strip_tac) >>
+ rw[isL_def] >> rpt strip_tac >>
+ first_assum match_mp_tac >> first_x_assum match_mp_tac >> arw[])
+(form_goal
+ “!A. isL(Empty(N * A))& 
+     (!nas:mem(Pow(N * A)). isL(nas) ==> 
+              !a. isL(Ins(Pair(CARD(nas),a),nas)))”));
+
+val isL_rules_step = isL_rules |> spec_all |> conjE2
+
+
+
+val isL_cases = prove_store("isL_cases",
+e0
+(strip_tac >> strip_tac >> dimp_tac >-- 
+ (qsuff_tac
+ ‘!nas. isL(nas) ==> (nas = Empty(N * A) |
+  (?nas0 a0. nas = Ins(Pair(CARD(nas0),a0),nas0) & isL(nas0)))’
+ >-- (strip_tac >> arw[]) >>
+ ind_with (isL_ind |> allE (rastt "A")) >> strip_tac (* 2 *)
+ >-- rw[] >>
+ rpt strip_tac (* 2 *) 
+ >-- (disj2_tac >> arw[] (*figure out why the arw work here*)>> 
+      qexistsl_tac [‘Empty(N * A)’,‘a’] >> 
+      rw[isL_rules]) >>
+ disj2_tac >> (*if arw[] >> here, then does not work*) 
+ qexistsl_tac [‘nas'’,‘a’] >> rw[] >> arw[] >>
+ match_mp_tac isL_rules_step >> arw[]) >>
+ rpt strip_tac (* 2 *)
+ >-- arw[isL_rules] >>
+ arw[] >> match_mp_tac isL_rules_step >> arw[])
+(form_goal
+ “!A nas. isL(nas) <=> (nas = Empty(N * A) |
+  (?nas0 a0. nas = Ins(Pair(CARD(nas0),a0),nas0) & isL(nas0)))”));
+
+
+
+
+val FI_cases = prove_store("FI_cases",
+e0
+(strip_tac >> strip_tac >> dimp_tac >-- 
+ (qsuff_tac
+ ‘!nas. isL(nas) ==> (nas = Empty(N * A) |
+  (?nas0 a0. nas = Ins(Pair(CARD(nas0),a0),nas0) & isL(nas0)))’
+ >-- (strip_tac >> arw[]) >>
+ ind_with (isL_ind |> allE (rastt "A")) >> strip_tac (* 2 *)
+ >-- rw[] >>
+ rpt strip_tac (* 2 *) 
+ >-- (disj2_tac >> arw[] rw[(assume “nas' = Empty(N * A)”)]
+     fconv_tac (top_depth_fconv 
+(rewr_conv (assume “nas' = Empty(N * A)”))
+no_fconv) >>
+
+ fconv_tac (basic_fconv 
+(rewr_conv (assume “nas' = Empty(N * A)”))
+no_fconv) 
+
+(*top_depth_fconv cannot, basic can do it.*)
+
+“Ins(Pair(CARD(nas':mem(Pow(N * A))), a:mem(A)), nas')”
+
+      
+
+
+arw[])))
+(form_goal
+ “!A nas. isL(nas) <=> (nas = Empty(N * A) |
+  (?nas0 a0. nas = Ins(Pair(CARD(nas0),a0),nas0) & isL(nas0)))”));
+
+
+
+(*
+top_depth_fconv 
+(first_conv 
+(List.map rewr_conv
+[assume “xs = xs':mem(Pow(X))”,
+ assume “n = n0:mem(N)”]))
+no_fconv
+“Cd(xs:mem(Pow(X)),n:mem(N))”
+
+top_depth_fconv 
+(first_conv 
+(List.map rewr_conv
+[assume “xs = xs':mem(Pow(X))”(*,
+ assume “n = n0:mem(N)” *)]))
+no_fconv
+“Cd(xs:mem(Pow(X)),n:mem(N))”
+
+
+top_depth_fconv 
+(rewr_conv (assume “nas' = Empty(N * A)”))
+no_fconv
+“Ins(Pair(CARD(nas':mem(Pow(N * A))), a:mem(A)), nas')”
+
+basic_fconv 
+(rewr_conv (assume “nas' = Empty(N * A)”))
+no_fconv
+“Ins(Pair(CARD(nas':mem(Pow(N * A))), a:mem(A)), nas')”
+
+because nas' is wrapped in some function which has one input...
+
+
+bugbugbug
+
+*)
+
+
+
+val FI_cases = val (ct,asl,w) = cg $
+e0
+(strip_tac >> strip_tac >> strip_tac >> dimp_tac >-- 
+ (qsuff_tac
+ ‘!xs n. Cd(xs,n) ==> ((xs = Empty(X) & n = O) |
+  (?xs0 n0 x0. ~(IN(x0,xs0)) & xs = Ins(x0,xs0) & n = Suc(n0) &
+  Cd(xs0,n0)))’
+ >-- (strip_tac >> arw[])))
+(form_goal
+ “!X xs:mem(Pow(X)) n. Cd(xs,n) <=> ((xs = Empty(X) & n = O) |
+  (?xs0 n0 x0. ~(IN(x0,xs0)) & xs = Ins(x0,xs0) & n = Suc(n0) &
+   Cd(xs0,n0)))”)
+
+
+
+
+(*
+alt of Cd_ind
+(form_goal 
+ “!X.(P(Pair(Empty(X),O)) &
+     (!xs n x:mem(X). 
+      P(Pair(xs,n)) & (~IN(x,xs)) ==> 
+      P(Pair(Ins(x,xs),Suc(n))))) ==>
+  !xs:mem(Pow(X)) n.Cd(xs,n) ==> P(xs,n)”))
+
+
+maybe use the idea that a subset of A * B is a subset of A and a subset of B, hence may turn the IN(Pair...) into IN(...,A) & IN(...,B)
+
+!(P : mem(Pow(Pow(X) * N))).
+               IN(Pair(Empty(X), O), P#) &
+               (!(xs0 : mem(Pow(X)))  (n0 : mem(N))  (x : mem(X)).
+                   IN(Pair(xs0#, n0#), P#) & ~IN(x#, xs0#) ==>
+                   IN(Pair(Ins(x#, xs0#), Suc(n0#)), P#)) ==>
+               IN(Pair(xs, n), P#)
+
+*)
+
+
+
+val f= “xs' = Ins(x0:mem(X), xs0)”
+val th = mk_thm(fvf f,[],f)
+
+basic_fconv (rewr_conv (assume “xs' = Ins(x0:mem(X), xs0)”))
+no_fconv
+“?xs0:mem(Pow(X)). Ins(x:mem(X),xs':mem(Pow(X)))”
+
+top_depth_fconv (rewr_conv (assume “xs' = Ins(x0:mem(X), xs0)”))
+no_fconv
+“?xs0:mem(Pow(X)). Ins(x:mem(X),xs':mem(Pow(X)))”
+
+
+
+top_depth_fconv (rewr_conv (assume “xs' = Ins(x0:mem(X), xs0)”))
+no_fconv
+“?xs0:mem(Pow(X)). Ins(x:mem(X),xs':mem(Pow(X))) = a”
+
+top_depth_conv (rewr_conv (assume “xs' = Ins(x0:mem(X), xs0)”))
+(rastt "Ins(x:mem(X),xs':mem(Pow(X)))")
+
+
+redepth_fconv (rewr_conv (assume “xs' = Ins(x0:mem(X), xs0)”))
+no_fconv
+“Ins(x:mem(X),xs':mem(Pow(X))) = a”
+
+
+arg_conv (rewr_conv (assume “xs' = Ins(x0:mem(X), xs0)”))
+(rastt "Ins(x:mem(X),xs':mem(Pow(X)))")
+
+arg_conv (try_conv (rewr_conv (assume “xs' = Ins(x0:mem(X), xs0)”)))
+(rastt "Ins(x:mem(X),xs':mem(Pow(X)))")
+
+
+The one in top_depth_conv does not have try_conv.Should I add it?
+
+
+
+(*
+
+val f= “xs' = Ins(x0:mem(X), xs0)”
+val th = mk_thm(fvf f,[],f)
+
+top_depth_fconv (rewr_conv th)
+no_fconv
+“Ins(x:mem(X),xs':mem(Pow(X))) = a”
+*)
+
+
+
+top_depth_fconv (rewr_conv th)
+no_fconv
+“?xs0:mem(Pow(X)). Ins(x:mem(X),xs':mem(Pow(X))) = a”
+
+
+
+basic_fconv (rewr_conv th)
+no_fconv
+“?xs0:mem(Pow(X)). Ins(x:mem(X),xs':mem(Pow(X)))”
+
+
+
+
+(*parser bug 
+“?xs0. Ins(x,xs')”
+
+parsed as 
+
+  (?(xs0 : set). Ins(x, xs')) 
+
+*)
+
+val inN_cases = prove_store("inN_cases",
+e0
+(strip_tac >> strip_tac >> dimp_tac >-- 
+ (qsuff_tac
+ ‘!xs. FI(xs) ==> (xs = Empty(X) |
+  (?xs0 x0. xs = Ins(x0,xs0) & FI(xs0)))’
+ >-- (strip_tac >> arw[]) >>
+ ind_with (FI_ind |> allE (rastt "X")) >> strip_tac (* 2 *)
+ >-- rw[] >>
+ rpt strip_tac (* 2 *) 
+ >-- (disj2_tac >> arw[] >> qexistsl_tac [‘Empty(X)’,‘x’] >> 
+     rw[FI_rules]) >>
+ disj2_tac >> arw[]
+
+
+qexists_tac ‘n0'’ >> rw[] >>
+ arw[] >> match_mp_tac inN_rules_step >> arw[]) >>
+ rpt strip_tac (* 2 *)
+ >-- arw[inN_rules] >>
+ arw[] >> match_mp_tac inN_rules_step >> arw[])
+(form_goal
+ “!X xs. FI(xs) <=> (xs = Empty(X) |
+  (?xs0 x0. xs = Ins(x0,xs0) & FI(xs0)))”));
+
+
+
+
+
+
+
+(*
+local 
+val l = allE (rastt "N0") IN_def_P_expand
+val inN_def_alt = prove_store("inN_def_alt",
+e0
+(strip_tac >> rw[inN_def] >> dimp_tac >> strip_tac >--
+ (qsuff_tac
+ ‘?P0. !n:mem(N0). IN(n,P0) <=> P(n)’
+ >-- (strip_tac >> 
+     first_x_assum (qspecl_then [‘P0’] assume_tac) >>
+     rfs[]) >>
+ strip_assume_tac l >> 
+ qexists_tac ‘s’ >> arw[]) >>
+ 
+ strip_tac >>
+ pop_assum (assume_tac o (spec_fVar “P(a) <=> IN(a,P)”))
+ strip_tac >> 
+qsuff_tac
+ ‘?P0. !n:mem(N0). IN(n,P0) <=> P(n)’
+ >-- (strip_tac >> 
+     first_x_assum (qspecl_then [‘P0’] assume_tac) >>
+     rfs[]) >>
+ strip_assume_tac l >> 
+ qexists_tac ‘s’ >> arw[] )
+(form_goal 
+     “!n. inN(n) <=> 
+    (P(O0) &
+     (!n0. P(n0) ==> P(Eval(S0,n0))) ==>
+     P(n))”))
+*)
